Printing.dfy
@@ -5,7 +5,7 @@ method printobject(o : Object)
 {
       printobj(o);
       print "\n  ";
-      printset(allExternalOwners(o));
+      printset(o.allExternalOwners());
       print "\n";
       printobjfields(o);
 }
@@ -86,6 +86,20 @@ method printobj(o : Object)
 }
 
 
+function fmtown(oo : Owner) : string 
+   reads oo
+{
+  "Own(" + fmtnickset(oo) + ")"
+}
+
+method printown(oo : Owner) 
+  ensures unchanged(oo)
+  modifies {}
+{
+ print fmtown(oo);
+}
+
+
 //should alos print field modes?
 method printobjfields(o : Object)
 {
@@ -137,7 +151,7 @@ method printmappingIsIsomorphic(m: Mapping, o : Object, os : set<Object>)
     print ":=";
     printobj(t[y]);
     print "  ";
-    print isIsomorphicMappingOWNED(y, o, m, os);
+//    print isIsomorphicMappingOWNED(y, o, m, os);
     print "\n";
     t := t - {y};
    }
@@ -151,68 +165,68 @@ method printmappingIsIsomorphic(m: Mapping, o : Object, os : set<Object>)
 
 
 
-method {:TRUMP} printIsomorphicOWNED(a : Object, o : Object, m : Mapping, os : set<Object>)
-  decreases os
+// method printIsomorphicOWNED(a : Object, o : Object, m : Mapping, os : set<Object>)
+//   decreases os
 
-  {
-   print "(a in m) ", (a in m), "\n"; 
-   if (a !in m) { return; }
-   var b := m[a];
-   print "a == b ", a == b, "\n";
-   if (a == b) { return; }
-   print "({a,b} <= os) ",({a,b} <= os),"\n";
-   //print "(m[a] == b) ", (m[a] == b), "\n";
-   print "(a.region.World? && b.region.World?) ", (a.region.World? && b.region.World?), "\n";
-   print "(a.region.Heap? && b.region.Heap?) ", (a.region.Heap? && b.region.Heap?), "\n";   
+//   {
+//    print "(a in m) ", (a in m), "\n"; 
+//    if (a !in m) { return; }
+//    var b := m[a];
+//    print "a == b ", a == b, "\n";
+//    if (a == b) { return; }
+//    print "({a,b} <= os) ",({a,b} <= os),"\n";
+//    //print "(m[a] == b) ", (m[a] == b), "\n";
 
-   if ((a.region.Heap?) && (b.region.Heap?)) {
-   print "(recurse on owner) ", isIsomorphicMappingOWNED(a.region.owner, o, m, os - {a,b}),"\n";
-   }  
+//    print "(recurse on owner) ", isIsomorphicMappingOWNED(a.owner, o, m, os - {a,b}),"\n";
 
-  print "Owners overall ", 
-    (|| (a.region.World? && b.region.World?) 
-     || ((a.region.Heap? && b.region.Heap?) && isIsomorphicMappingOWNED(a.region.owner, o, m, os - {a,b})))
-  ,"\n";
+//   print "Owners overall ", 
+//     isIsomorphicMappingOWNED(a.owner, o, m, os - {a,b}) ,"\n";
 
-  print "Field names ", (a.fields.Keys == b.fields.Keys), "\n";
+//   print "Field names ", (a.fields.Keys == b.fields.Keys), "\n";
 
-  if (a.fields.Keys != b.fields.Keys) { 
-      print "oops! a: ", a.fields.Keys,"\n";
-      print "oops! b: ", b.fields.Keys,"\n";
-      return; }
+//   if (a.fields.Keys != b.fields.Keys) { 
+//       print "oops! a: ", a.fields.Keys,"\n";
+//       print "oops! b: ", b.fields.Keys,"\n";
+//       return; }
 
-  var ns : seq<string> := set2seq(a.fields.Keys);
+//   var ns : seq<string> := set2seq(a.fields.Keys);
 
-  for i := 0 to |ns| 
-   {
-    var n : string := ns[i];
-    print "  ";
-    print "a.",n," :=";
-    printobj(a.fields[n]);
-    print " - ";
-    print "b.",n," :=";
-    printobj(b.fields[n]);
-    print "\n";
+//   for i := 0 to |ns| 
+//    {
+//     var n : string := ns[i];
+//     print "  ";
+//     print "a.",n," :=";
+//     printobj(a.fields[n]);
+//     print " - ";
+//     print "b.",n," :=";
+//     printobj(b.fields[n]);
+//     print "\n";
 
-    print "   a.",n," in m ", a.fields[n] in m, "\n";
-    if (a.fields[n] !in m) {return;}
-    print "   ",n," in b.fields ", n in b.fields, "\n";
-    if (n !in b.fields) {return;}
-    print "   b.fields[",n,"] == m[a.fields[",n,"]] ",(b.fields[n] == m[a.fields[n]]) , "\n";
-    print " (recurse on field ",n,") ", isIsomorphicMappingOWNED(a.fields[n], o, m, os - {a,b}),"\n";
-   }
-}
-
-function {:onlyfans} fmtseqstr(ss : seq<string>) : string 
-decreases ss
-{
-  if (|ss| == 0) then ("")
-  else (if (|ss| == 1) then (ss[0])
-  else (ss[0] + "," + fmtseqstr(ss[1..]))
-  )
-}
+//     print "   a.",n," in m ", a.fields[n] in m, "\n";
+//     if (a.fields[n] !in m) {return;}
+//     print "   ",n," in b.fields ", n in b.fields, "\n";
+//     if (n !in b.fields) {return;}
+//     print "   b.fields[",n,"] == m[a.fields[",n,"]] ",(b.fields[n] == m[a.fields[n]]) , "\n";
+// //    print " (recurse on field ",n,") ", isIsomorphicMappingOWNED(a.fields[n], o, m, os - {a,b}),"\n";
+//    }
+// }
 
 
 
 
+function fmtnickset(Y: set<Object>) : string
+ {
+  //var Y := X;
+  if (Y == {}) then ("") else (
+      var y : Object :| y in Y && (forall z <- Y :: y.nick <= z.nick );
+      y.nick + " " + fmtnickset( Y - {y} ) )
+  } 
 
+
+
+function fmtseqstr(Y: seq<string>) : string  //isnt this just a flatten?
+ {
+  //var Y := X;
+  if (Y == []) then ("") else (
+       Y[0] + " " + fmtseqstr( Y[1..] ) )
+  } 
